new, generic indexing approach

secure_api/box/Box.Index.fst
@@ -7,206 +7,238 @@ open FStar.Endianness
 
 module MM = FStar.Monotonic.Map
 
-let id_length = 32
-
-type cipherAlg =
-  | A
-  | B
-
-type pk = lbytes id_length
-type id =
-  | PK_id of pk
-  | Instance_id of (id:(pk*pk))
-
-let pk_id = i:id{PK_id? i}
-let inst_id = i:id{Instance_id? i}
-
-val compose_id: i1:pk_id -> i2:pk_id{i1 <> i2} -> i:inst_id
-let compose_id i1 i2 =
-  let i1,i2 =
-    match i1,i2 with
-    | PK_id i1,PK_id i2 -> i1,i2
-  in
-  let int_i1 = little_endian i1 in
-  let int_i2 = little_endian i2 in
-  if int_i1 < int_i2 then
-    Instance_id (i1,i2)
-  else
-    Instance_id (i2,i1)
-
-#set-options "--z3rlimit 300 --max_ifuel 1 --max_fuel 1"
-val lemma_symmetric_id:  i1:pk_id -> i2:pk_id{i1 <> i2} -> Lemma
-  (requires True)
-  (ensures compose_id i1 i2 = compose_id i2 i1)
-  [SMTPat (compose_id i1 i2)]
-let lemma_symmetric_id i1 i2 =
-  let i1,i2 =
-    match i1,i2 with
-    | PK_id i1,PK_id i2 -> i1,i2
-  in
-  lemma_little_endian_bij i1 i2
-
-
-type index_log_key = i:pk_id
+#set-options "--z3rlimit 300 --max_ifuel 2 --max_fuel 1"
+let index_log_key (t:Type0{hasEq t}) = i:t
 let index_log_value = bool
-let index_log_range (k:index_log_key) = index_log_value
-let index_log_inv (f:MM.map' (index_log_key) (index_log_range)) = True
+let index_log_range (#t:Type0{hasEq t}) (k:index_log_key t) = index_log_value
+let index_log_inv (#t:Type0{hasEq t}) (f:MM.map' (index_log_key t) (index_log_range)) = True
 
-let index_log (rgn:erid) =
-  MM.t rgn (index_log_key) (index_log_range) (index_log_inv)
+let index_log (t:Type0{hasEq t}) (rgn:erid) =
+  MM.t rgn (index_log_key t) (index_log_range) (index_log_inv)
 
-noeq type index_package =
-  | IP:
-  id_log_rgn : erid ->
-  id_log: index_log id_log_rgn ->
-  index_package
+noeq
+type index_package =
+  | Leaf_IP:
+    t:eqtype u#0 ->
+    rgn : erid ->
+    log: index_log t rgn ->
+    index_package
+  | Node_IP:
+    children:list index_package{children =!= []} ->
+    index_package
 
-val create_index_package: rgn:erid -> ST (index_package)
+val id: ip:index_package -> eqtype u#0
+val unfold_id: l:list index_package{l =!= []} -> eqtype u#0
+
+let rec id ip =
+  match ip with
+  | Leaf_IP t _ _ -> t
+  | Node_IP ips -> unfold_id ips
+and unfold_id = function
+  | [ip] -> id ip
+  | hd :: tl -> id hd * unfold_id tl
+
+type logical_operator =
+  | CONJ
+  | DISJ
+
+val apply_predicate: #ip:index_package -> i:id ip -> predicate:(#rgn:erid -> #t:eqtype -> i:t -> index_log t rgn -> Type0) -> op:logical_operator -> t:Type0
+val all_apply_predicate: #ips:list index_package{Nil? ips = false} -> unfold_id ips -> (#rgn:erid -> #t:eqtype -> i:t -> index_log t rgn -> Type0) -> op:logical_operator -> Type0
+
+let rec apply_predicate #ip x predicate op =
+  match ip with
+  | Leaf_IP t rgn log -> predicate #rgn #t x log
+  | Node_IP childs -> all_apply_predicate #childs x predicate op
+and all_apply_predicate #ips x predicate op =
+  match ips with
+  | [ip'] -> apply_predicate #ip' x predicate op
+  | ip' :: tl ->
+    let v, vs : id ip' * unfold_id tl = x in
+    match op with
+    | CONJ -> apply_predicate v predicate op /\ all_apply_predicate vs predicate op
+    | DISJ -> apply_predicate v predicate op \/ all_apply_predicate vs predicate op
+
+
+private let fresh_predicate =
+  fun (h:mem)
+    (#rgn:erid)
+    (#t:eqtype)
+    (i:t)
+    (log:index_log t rgn) ->
+    MM.fresh log i h
+val fresh: #ip:index_package -> i:id ip -> h:mem -> Type0
+let fresh #ip i h =
+  apply_predicate i (fresh_predicate h) CONJ
+
+private let registered_predicate =
+  fun (#rgn:erid)
+    (#t:eqtype)
+    (i:t)
+    (log:index_log t rgn) ->
+    witnessed (MM.defined log i)
+val registered: #ip:index_package -> i:id ip -> t:Type0{
+  t /\ Leaf_IP? ip ==>
+  (match ip with
+  | Leaf_IP t rgn log -> witnessed (MM.defined log i))
+  }
+let registered #ip i =
+  apply_predicate i registered_predicate CONJ
+
+private let honest_predicate =
+  fun (#rgn:erid)
+    (#t:eqtype)
+    (i:t)
+    (log:index_log t rgn) ->
+    witnessed (MM.contains log i true)
+val honest: #ip:index_package -> i:id ip -> Type0
+let honest #ip i =
+  apply_predicate i honest_predicate CONJ
+
+private let corrupt_predicate =
+  fun (#rgn:erid)
+    (#t:eqtype)
+    (i:t)
+    (log:index_log t rgn) ->
+    witnessed (MM.contains log i false)
+val corrupt: #ip:index_package -> i:id ip -> Type0
+let corrupt #ip i =
+  apply_predicate i corrupt_predicate DISJ
+
+val create_leaf_index_package: rgn:erid -> t:Type0{hasEq t} -> ST (ip:index_package{Leaf_IP? ip})
   (requires (fun h0 -> True))
   (ensures (fun h0 ip h1 ->
-    modifies (Set.singleton rgn) h0 h1
-    /\ contains h1 ip.id_log
+    match ip with
+    | Leaf_IP t' rgn' log ->
+    t == t'
+    /\ modifies (Set.singleton rgn) h0 h1
+    /\ extends rgn' rgn
+    /\ contains h1 log
+    /\ (forall i . fresh #ip i h1)
   ))
-let create_index_package rgn =
+let create_leaf_index_package rgn t =
   let log_rgn = new_region rgn in
-  let log = MM.alloc #log_rgn #index_log_key #index_log_range #index_log_inv in
-  IP log_rgn log
+  let log = MM.alloc #log_rgn #(index_log_key t) #(index_log_range #t) #index_log_inv in
+  Leaf_IP t log_rgn log
 
-val fresh: ip:index_package -> i:pk_id -> h:mem -> Type0
-let fresh ip i h =
-  MM.fresh ip.id_log i h
-  //match i with
-  //| PK_id i' -> MM.fresh ip.id_log (PK_id i') h
-  //| Instance_id i' -> MM.fresh ip.id_log (PK_id (fst i')) h \/ MM.fresh ip.id_log (PK_id (snd i')) h
+val create_node_index_package: l:list index_package{l =!= []} -> ST (ip:index_package{Node_IP? ip})
+  (requires (fun h0 -> True))
+  (ensures (fun h0 ip h1 ->
+    h0 == h1
+  ))
+let create_node_index_package l =
+  Node_IP l
 
-val registered: ip:index_package -> i:id -> Type0
-let registered ip i =
-  match i with
-  | PK_id i' -> witnessed (MM.defined ip.id_log (PK_id i'))
-  | Instance_id i' -> witnessed (MM.defined ip.id_log (PK_id (fst i'))) /\ witnessed (MM.defined ip.id_log (PK_id (snd i')))
+val extend_id_log: (#ip:index_package{Leaf_IP? ip}) -> (i:id ip) -> (b:bool) -> (h0:mem) -> (h1:mem) -> Type0
+let extend_id_log #ip i b h0 h1 =
+  match ip with
+  | Leaf_IP t rgn log ->
+    (sel h1 log == MM.upd (sel h0 log) i b
+    /\ witnessed (MM.defined log i)
+    /\ witnessed (MM.contains log i b)
+    )
 
-#set-options "--z3rlimit 300 --max_ifuel 2 --max_fuel 1"
-val honest: ip:index_package -> i:id -> t:Type0//{t ==> PK_id? i ==> registered_pk ip i}
-let honest ip i =
-  match i with
-  | PK_id i' ->
-    witnessed (MM.contains ip.id_log (PK_id i') true)
-  | Instance_id i' -> witnessed (MM.contains ip.id_log (PK_id (fst i')) true) /\ witnessed (MM.contains ip.id_log (PK_id (snd i')) true)
+let register_footprint (ip:index_package{Leaf_IP? ip}) (h0:mem) (h1:mem) =
+  match ip with
+  | Leaf_IP t rgn log ->
+    modifies (Set.singleton rgn) h0 h1
 
-val dishonest: ip:index_package -> i:id -> Type0
-let dishonest ip i =
-  match i with
-  | PK_id i' ->
-    witnessed (MM.contains ip.id_log (PK_id i') false)
-  | Instance_id i' -> witnessed (MM.contains ip.id_log (PK_id (fst i')) false) \/ witnessed (MM.contains ip.id_log (PK_id (snd i')) false)
-
-let extend_id_log (ip:index_package) (i:pk_id) (b:bool) (h0:mem) (h1:mem) =
-  (sel h1 ip.id_log == MM.upd (sel h0 ip.id_log) i b
-  /\ witnessed (MM.defined ip.id_log i)
-  /\ witnessed (MM.contains ip.id_log i b))
-
-let register_footprint (ip:index_package) (h0:mem) (h1:mem) =
-  modifies (Set.singleton ip.id_log_rgn) h0 h1
-
-val register: ip:index_package -> i:pk_id -> b:bool -> ST unit
+val register: #ip:index_package{Leaf_IP? ip} -> i:id ip -> b:bool -> ST unit
   (requires (fun h0 ->
-    MM.fresh ip.id_log i h0
+    fresh i h0
   ))
   (ensures (fun h0 _ h1 ->
-    (b ==> honest ip i)
-    /\ (~b ==> dishonest ip i)
-    /\ extend_id_log ip i b h0 h1
+    extend_id_log i b h0 h1
+    /\ (b ==> honest i)
+    /\ (~b ==> corrupt i)
+    /\ registered i
     /\ register_footprint ip h0 h1
   ))
-let register ip i b =
-  MM.extend ip.id_log i b
+let register #ip i b =
+  match ip with
+  | Leaf_IP t rgn log ->
+    MM.extend log i b;
+    assert(b ==> apply_predicate i honest_predicate CONJ);
+    assert(~b ==> apply_predicate i corrupt_predicate DISJ)
 
-
-#set-options "--z3rlimit 300 --max_ifuel 3 --max_fuel 3"
-val get_honesty: ip:index_package -> i:id -> ST bool
+#set-options "--z3rlimit 300 --max_ifuel 1 --max_fuel 1"
+val get_honesty: #ip:index_package -> i:id ip -> ST bool
   (requires (fun h0 ->
-    registered ip i
+    registered i
   ))
   (ensures (fun h0 b h1 ->
     h0 == h1
-    /\ ((b2t b) ==> honest ip i)
-    /\ (~(b2t b) ==> dishonest ip i)
-    /\ (PK_id? i ==> MM.contains ip.id_log i b h0)
+    /\ ((b2t b) ==> honest i)
+    /\ (~(b2t b) ==> corrupt i)
   ))
-let rec get_honesty ip i =
-  match i with
-  | PK_id i' ->
-    testify (MM.defined ip.id_log (PK_id i'));
-    (match MM.lookup ip.id_log i with
+val all_get_honesty: #ips:list index_package{ips =!= []} -> i:unfold_id ips -> ST bool
+  (requires (fun h0 ->
+    all_apply_predicate #ips i registered_predicate CONJ
+  ))
+  (ensures (fun h0 b h1 ->
+    h0 == h1
+    /\ (b2t b ==> all_apply_predicate #ips i honest_predicate CONJ)
+    /\ (~(b2t b) ==> all_apply_predicate #ips i corrupt_predicate DISJ)
+  ))
+let rec get_honesty #ip i =
+  match ip with
+  | Leaf_IP t rgn log ->
+    testify (MM.defined log i);
+    (match MM.lookup log i with
     | Some b -> (
       (if b then
-        testify (MM.contains ip.id_log i true)
+        testify (MM.contains log i true)
       else
-        testify (MM.contains ip.id_log i false));
+        testify (MM.contains log i false));
+      assert(b2t b ==> apply_predicate i honest_predicate CONJ);
+      assert(~(b2t b) ==> apply_predicate i corrupt_predicate DISJ);
       b))
-  | Instance_id i' ->
-    let b1 = get_honesty ip (PK_id (fst i')) in
-    let b2 = get_honesty ip (PK_id (snd i')) in
+  | Node_IP ips ->
+    let b = all_get_honesty #ips i in
+    assert(b2t b ==> all_apply_predicate #ips i honest_predicate CONJ);
+    assert(~(b2t b) ==> all_apply_predicate #ips i corrupt_predicate DISJ);
+    b
+and all_get_honesty #ips i =
+  match ips with
+  | [ip'] -> get_honesty #ip' i
+  | ip' :: tl ->
+    let v, vs : id ip' * unfold_id tl = i in
+    let b1 = get_honesty #ip' v in
+    assert(b2t b1 ==> apply_predicate #ip' v honest_predicate CONJ);
+    assert(~(b2t b1) ==> apply_predicate #ip' v corrupt_predicate DISJ);
+    let b2 = all_get_honesty #tl vs in
+    assert(b2t b2 ==> all_apply_predicate #tl vs honest_predicate CONJ);
+    assert(~(b2t b2) ==> all_apply_predicate #tl vs corrupt_predicate DISJ);
     b1 && b2
 
-type absurd_honest (ip:index_package) (i:id{dishonest ip i}) = honest ip i
-type absurd_dishonest (ip:index_package) (i:id{honest ip i}) = dishonest ip i
-assume val lemma_honest_and_others_tot: ip:index_package -> i:id{dishonest ip i} -> absurd_honest ip i -> Lemma (False)
-assume val lemma_dishonest_and_others_tot: ip:index_package -> i:id{honest ip i} -> absurd_dishonest ip i -> Lemma (False)
+
+type absurd_honest (#ip:index_package) (i:id ip{corrupt i}) = honest i
+type absurd_corrupt (#ip:index_package) (i:id ip{honest i}) = corrupt i
+assume val lemma_honest_and_others_tot: #ip:index_package -> i:id ip{corrupt i} -> absurd_honest i -> Lemma (False)
+assume val lemma_corrupt_and_others_tot: #ip:index_package -> i:id ip{honest i} -> absurd_corrupt i -> Lemma (False)
 
 
-val lemma_dishonest_not_others: ip:index_package -> (i:id) -> Lemma
+val lemma_corrupt_not_others: #ip:index_package -> (i:id ip) -> Lemma
   (requires (
-    dishonest ip i
+    corrupt i
   ))
   (ensures (
-    ~(honest ip i)
+    ~(honest i)
   ))
-  [SMTPat (dishonest ip i)]
-let lemma_dishonest_not_others ip i =
-  let (j:(i:id{dishonest ip i})) = i in
-  FStar.Classical.impl_intro (lemma_honest_and_others_tot ip j);
-  assert(honest ip i==> False)
+  [SMTPat (corrupt i)]
+let lemma_corrupt_not_others #ip i =
+  let (j:(i:id ip{corrupt i})) = i in
+  FStar.Classical.impl_intro (lemma_honest_and_others_tot j);
+  assert(honest i==> False)
 
-val lemma_honest_not_others: ip:index_package -> (i:id) -> Lemma
+val lemma_honest_not_others: #ip:index_package -> (i:id ip) -> Lemma
   (requires (
-    honest ip i
+    honest i
   ))
   (ensures (
-    ~(dishonest ip i)
+    ~(corrupt i)
   ))
-  [SMTPat (honest ip i)]
-let lemma_honest_not_others ip i =
-  let (j:(i:id{honest ip i})) = i in
-  FStar.Classical.impl_intro (lemma_dishonest_and_others_tot ip j);
-  assert(dishonest ip i ==> False)
-
-
-//val lemma_honest_or_dishonest: ip:index_package -> (i:id) -> Lemma
-//  (requires (
-//    registered ip i
-//  ))
-//  (ensures (
-//    ~(dishonest ip i)
-//  ))
-//  [SMTPat (honest ip i)]
-//let lemma_honest_or_dishonest ip i =
-//  let (j:(i:id{honest ip i})) = i in
-//  FStar.Classical.impl_intro (lemma_dishonest_and_others_tot ip j);
-//  assert(dishonest ip i ==> False)
-
-//val lemma_honest_dishonest: ip:index_package -> i:id -> ST unit
-//  (requires (fun h0 ->
-//    ~(honest ip i) /\ registered ip i
-//  ))
-//  (ensures (fun h0 _ h1 ->
-//    (dishonest ip i)
-//  ))
-//let rec lemma_honest_dishonest ip i =
-//  match i with
-//  | PK_id i' -> testify (MM.defined ip.id_log (PK_id i'));
-//    (match MM.lookup ip.id_log i with
-//    | Some b -> assert(b = false))
-//  | Instance_id i' ->
-//    lemma_honest_dishonest ip (PK_id (fst i'));
-//    lemma_honest_dishonest ip (PK_id (snd i'))
+  [SMTPat (honest i)]
+let lemma_honest_not_others #ip i =
+  let (j:(i:id ip{honest i})) = i in
+  FStar.Classical.impl_intro (lemma_corrupt_and_others_tot j);
+  assert(corrupt i ==> False)
